ArkLib/ToMathlib/Data/IndexedBinaryTree/Equiv.lean
@@ -1,0 +1,95 @@
+import ArkLib.ToMathlib.Data.IndexedBinaryTree.Basic
+
+
+/-!
+# Equivalences
+
+This section contains theorems about equivalences between different tree indexing types
+and data structures.
+-/
+
+namespace BinaryTree
+
+section Equivalences
+
+/-- `LeafData`s are equivalent to functions from `SkeletonLeafIndex` to values -/
+def LeafData.EquivIndexFun {α : Type} (s : Skeleton) :
+    LeafData α s ≃ (SkeletonLeafIndex s → α) where
+  toFun := fun tree idx => tree.get idx
+  invFun := sorry
+  left_inv := sorry
+  right_inv := sorry
+
+/-- `InternalData`s are equivalent to functions from `SkeletonInternalIndex` to values -/
+def InternalData.EquivIndexFun {α : Type} (s : Skeleton) :
+    InternalData α s ≃ (SkeletonInternalIndex s → α) where
+  toFun := fun tree idx => tree.get idx
+  invFun := sorry
+  left_inv := sorry
+  right_inv := sorry
+
+/-- `FullData`s are equivalent to functions from `SkeletonNodeIndex` to values -/
+def FullData.EquivIndexFun {α : Type} (s : Skeleton) :
+    FullData α s ≃ (SkeletonNodeIndex s → α) where
+  toFun := fun tree idx => tree.get idx
+  invFun := sorry
+  left_inv := sorry
+  right_inv := sorry
+
+/-- A `LeafData` can be interpreted as a function from `SkeletonLeafIndex` to values -/
+instance {α : Type} {s : Skeleton} :
+    CoeFun (LeafData α s) fun (_ : LeafData α s) => SkeletonLeafIndex s → α where
+  coe := fun tree idx => tree.get idx
+
+/-- An `InternalData` can be interpreted as a function from `SkeletonInternalIndex` to values -/
+instance {α : Type} {s : Skeleton} :
+    CoeFun (InternalData α s) fun (_ : InternalData α s) => SkeletonInternalIndex s → α where
+  coe := fun tree idx => tree.get idx
+
+/-- A `FullData` can be interpreted as a function from `SkeletonNodeIndex` to values -/
+instance {α : Type} {s : Skeleton} :
+    CoeFun (FullData α s) fun (_ : FullData α s) => SkeletonNodeIndex s → α where
+  coe := fun tree idx => tree.get idx
+
+/--
+A function taking a `SkeletonNodeIndex s`
+to either a `SkeletonInternalIndex s` or a `SkeletonLeafIndex s`
+-/
+def SkeletonNodeIndex.toSum {s : Skeleton} :
+    SkeletonNodeIndex s → SkeletonInternalIndex s ⊕ SkeletonLeafIndex s :=
+  fun idx =>
+    match idx with
+    | SkeletonNodeIndex.ofLeaf => Sum.inr (SkeletonLeafIndex.ofLeaf)
+    | SkeletonNodeIndex.ofInternal => Sum.inl (SkeletonInternalIndex.ofInternal)
+    | SkeletonNodeIndex.ofLeft idxLeft => match idxLeft.toSum with
+      | .inl idxLeft => Sum.inl (SkeletonInternalIndex.ofLeft idxLeft)
+      | .inr idxLeft => Sum.inr (SkeletonLeafIndex.ofLeft idxLeft)
+    | SkeletonNodeIndex.ofRight idxRight => match idxRight.toSum with
+      | .inl idxRight => Sum.inl (SkeletonInternalIndex.ofRight idxRight)
+      | .inr idxRight => Sum.inr (SkeletonLeafIndex.ofRight idxRight)
+
+/-- Equivalence between node indices and the sum of internal and leaf indices -/
+def SkeletonNodeIndex.SumEquiv (s : Skeleton) :
+    SkeletonInternalIndex s ⊕ SkeletonLeafIndex s ≃ SkeletonNodeIndex s :=
+{
+  toFun x := match x with
+    | Sum.inl idx => idx.toNodeIndex
+    | Sum.inr idx => idx.toNodeIndex,
+  invFun idx := idx.toSum,
+  left_inv := sorry,
+  right_inv := sorry,
+}
+
+/-- Equivalence between `FullData` and the product of `InternalData` and `LeafData` -/
+def FullData.Equiv {α} (s : Skeleton) :
+    FullData α s ≃ InternalData α s × LeafData α s := by
+  calc
+    FullData α s ≃ (SkeletonNodeIndex s → α) := FullData.EquivIndexFun s
+    _ ≃ (SkeletonInternalIndex s ⊕ SkeletonLeafIndex s → α) := by sorry
+    _ ≃ (SkeletonInternalIndex s → α) × (SkeletonLeafIndex s → α) := by sorry
+    _ ≃ InternalData α s × LeafData α s := by sorry
+
+
+end Equivalences
+
+end BinaryTree
