ArkLib/ToMathlib/Data/IndexedBinaryTree/Lemmas.lean
@@ -1,0 +1,64 @@
+import ArkLib.ToMathlib.Data.IndexedBinaryTree.Basic
+
+
+/-!
+# Lemmas about Indexed Binary Trees
+
+## TODOs
+
+- More relationships between tree navigations
+  - Which navigation sequences are equivalent to each other?
+  - How do these navigations affect depth?
+- API for flattening a tree to a list
+- Define `Lattice` structure on trees
+  - a subset relation on trees, mappings of indices to indices of supertrees
+
+
+-/
+
+namespace BinaryTree
+
+section Navigation
+
+/-- The parent of a leftChild is none or the node -/
+theorem SkeletonNodeIndex.leftChild_bind_parent {s : Skeleton}
+    (idx : SkeletonNodeIndex s) :
+    idx.leftChild >>= parent = (if idx.isLeaf then none else some idx) := by
+  sorry
+
+/-- The parent of a rightChild is none or the node -/
+theorem SkeletonNodeIndex.rightChild_bind_parent {s : Skeleton}
+    (idx : SkeletonNodeIndex s) :
+    idx.rightChild >>= parent = (if idx.isLeaf then none else some idx) := by
+  sorry
+
+/-- The parent of a leftChild is none or the node -/
+
+theorem SkeletonNodeIndex.parent_of_depth_zero {s : Skeleton}
+    (idx : SkeletonNodeIndex s) (h : idx.depth = 0) :
+    parent idx = none := by
+  cases idx with
+  | ofLeaf => rfl
+  | ofInternal => rfl
+  | ofLeft idxLeft =>
+    unfold depth at h
+    simp_all
+  | ofRight idxRight =>
+    unfold depth at h
+    simp_all
+
+-- TODO?: reorder the arguments to `LeafData` etc. so that the skeleton comes first?
+
+instance {s} : Functor (fun α => LeafData α s) where
+  map f x := x.map f
+
+instance {s} : Functor (fun α => InternalData α s) where
+  map f x := x.map f
+
+instance {s} : Functor (fun α => FullData α s) where
+  map f x := x.map f
+
+
+instance {s} : LawfulFunctor (fun α => LeafData α s) := by sorry
+instance {s} : LawfulFunctor (fun α => InternalData α s) := by sorry
+instance {s} : LawfulFunctor (fun α => FullData α s) := by sorry
